

Given, sample data are

$$X = \{x_{ij} : 1 \leq i \leq k, 1 \leq j \leq n_i\}$$

$$\& \bar{x} = \text{mean}(X) = \frac{1}{n} \sum_{i=1}^k \sum_{j=1}^{n_i} x_{ij}$$

$$\text{Let } \bar{x}_i = \frac{1}{n_i} \sum_{j=1}^{n_i} x_{ij}$$

Hence

$$\begin{aligned} & \sum_{i=1}^k \sum_{j=1}^{n_i} (x_{ij} - \bar{x})^2 \\ &= \sum_{i=1}^k \sum_{j=1}^{n_i} ((x_{ij} - \bar{x}_i) + (\bar{x}_i - \bar{x}))^2 \\ &= \sum_{i=1}^k \sum_{j=1}^{n_i} (x_{ij} - \bar{x}_i)^2 + (\bar{x}_i - \bar{x})^2 + 2(x_{ij} - \bar{x}_i)(\bar{x}_i - \bar{x}) \end{aligned}$$

But observe,

$$\begin{aligned} \sum_{i=1}^k \sum_{j=1}^{n_i} (x_{ij} - \bar{x}_i) &= SSE \quad \& \quad \sum_{i=1}^k \sum_{j=1}^{n_i} (\bar{x}_i - \bar{x})^2 \\ &= \sum_{i=1}^k n_i (\bar{x}_i - \bar{x})^2 \\ &= SST \quad \text{[As summand is independent of } j \text{]} \end{aligned}$$

$$\begin{aligned} \text{Finally, } & \sum_{i=1}^k \sum_{j=1}^{n_i} (x_{ij} - \bar{x}_i)(\bar{x}_i - \bar{x}) \\ &= \sum_{i=1}^k \left(\sum_{j=1}^{n_i} x_{ij} (\bar{x}_i - \bar{x}) + \sum_{j=1}^{n_i} \bar{x}_i (\bar{x}_i - \bar{x}) \right) \\ &= \sum_{i=1}^k \left(\left(\sum_{j=1}^{n_i} x_{ij} - n_i \bar{x}_i \right) (\bar{x}_i - \bar{x}) \right) \quad \text{[As } \bar{x}_i - \bar{x} \text{ is ind. of } j \text{]} \\ &= \sum_{i=1}^k (n_i \bar{x}_i - n_i \bar{x}_i) (\bar{x}_i - \bar{x}) \quad \text{[By defn]} \\ &= \sum_{i=1}^k 0 (\bar{x}_i - \bar{x}) = 0. \end{aligned}$$

Hence, adding everything up, we get

$$\sum_{i=1}^n \sum_{j=1}^{n_i} (x_{ij} - \bar{x})^2 = SSE + SST + 0$$

$$= SSE + SST$$

as derived

[Note: this is very much similar to law of total variance, also called law of conditional variance, that is

$$\text{Var}(X) = E(\text{Var}(X|Y)) + \text{Var}(E(X|Y))$$

↑
corresponds to
SSE

↑
corresponds to
SST